books/centaur/fgl/pathcond-aignet.lisp
@@ -1,0 +1,330 @@
+; GL - A Symbolic Simulation Framework for ACL2
+; Copyright (C) 2008-2013 Centaur Technology
+;
+; Contact:
+;   Centaur Technology Formal Verification Group
+;   7600-C N. Capital of Texas Highway, Suite 300, Austin, TX 78731, USA.
+;   http://www.centtech.com/
+;
+; License: (An MIT/X11-style license)
+;
+;   Permission is hereby granted, free of charge, to any person obtaining a
+;   copy of this software and associated documentation files (the "Software"),
+;   to deal in the Software without restriction, including without limitation
+;   the rights to use, copy, modify, merge, publish, distribute, sublicense,
+;   and/or sell copies of the Software, and to permit persons to whom the
+;   Software is furnished to do so, subject to the following conditions:
+;
+;   The above copyright notice and this permission notice shall be included in
+;   all copies or substantial portions of the Software.
+;
+;   THE SOFTWARE IS PROVIDED "AS IS", WITHOUT WARRANTY OF ANY KIND, EXPRESS OR
+;   IMPLIED, INCLUDING BUT NOT LIMITED TO THE WARRANTIES OF MERCHANTABILITY,
+;   FITNESS FOR A PARTICULAR PURPOSE AND NONINFRINGEMENT. IN NO EVENT SHALL THE
+;   AUTHORS OR COPYRIGHT HOLDERS BE LIABLE FOR ANY CLAIM, DAMAGES OR OTHER
+;   LIABILITY, WHETHER IN AN ACTION OF CONTRACT, TORT OR OTHERWISE, ARISING
+;   FROM, OUT OF OR IN CONNECTION WITH THE SOFTWARE OR THE USE OR OTHER
+;   DEALINGS IN THE SOFTWARE.
+;
+; Original author: Sol Swords <sswords@centtech.com>
+ 
+(in-package "AIGNET")
+
+(include-book "centaur/aignet/mark-impls" :dir :system)
+(include-book "centaur/misc/intstack" :dir :system)
+(include-book "centaur/aignet/semantics" :dir :system)
+(local (include-book "theory"))
+(local (std::add-default-post-define-hook :fix))
+
+(acl2::defstobj-clone pathcond-nodebits acl2::bitarr :prefix "PATHCOND-")
+(acl2::defstobj-clone pathcond-nodestack acl2::intstack :prefix "PATHCOND-")
+(acl2::defstobj-clone pathcond-memo eba :prefix "PCMEMO-")
+;; (acl2::defstobj-clone pathcond-memo0 eba :prefix "PCMEMO0-")
+
+
+(local (in-theory (disable lookup-id-out-of-bounds
+                           lookup-id-in-bounds-when-positive)))
+
+(local (in-theory (enable aignet-idp)))
+
+(fty::defalist node-bit-alist :key-type natp :val-type bitp :true-listp t)
+
+(define nbalistp (x)
+  (and (node-bit-alistp x)
+       (no-duplicatesp-equal (alist-keys x)))
+  ///
+  (defthm nbalistp-of-cons
+    (implies (and (nbalistp 
+
+
+(defstobj aignet-pathcond$c
+  (pathcond-nodebits$c :type bitarr)
+  (pathcond-nodestack$c :type acl2::intstack))
+
+
+(define aignet-pathcond-lookup ((id natp)
+                                pathcond-nodebits
+                                pathcond-nodestack)
+  :guard (< id (bits-length pathcond-nodebits))
+  :returns (ans acl2::maybe-bitp :rule-classes :type-prescription)
+  (and (acl2::intstack-member id pathcond-nodestack)
+       (get-bit id pathcond-nodebits)))
+
+(define aignet-pathcond-push ((id natp)
+                              (val bitp)
+                              pathcond-nodebits
+                              pathcond-nodestack)
+  :guard (not (acl2::intstack-member id pathcond-nodestack))
+  :returns (mv new-pathcond-nodebits
+               new-pathcond-nodestack)
+  (b* ((pathcond-nodestack (acl2::intstack-push id pathond-nodestack))
+       (pathcond-nodebits (set-bit id val pathcond-nodebits)))
+    (mv pathcond-nodebits pathcond-nodestack)))
+  
+
+(defsection aignet-pathcond-eval
+  (defun-sk aignet-pathcond-eval (aignet
+                                  pathcond-nodebits
+                                  pathcond-nodestack
+                                  invals regvals)
+    (forall id 
+            (implies (member id pathcond-nodestack)
+                     (equal (nth id pathcond-nodebits)
+                            (acl2::id-eval id invals regvals aignet))))
+    :rewrite :direct)
+
+  
+
+  )
+
+
+
+
+(defconst *aignet-pathcond-implies-template*
+  ;; Dumb template so we don't have to write this body twice in slightly different variants.
+  ;; Substitutions: 
+  ;; fnname: obvious
+  ;; memo-args: memo tables to pass around
+  ;; returns: :returns entry
+  ;; memo-guard: list of conjuncts for guard of memo-args
+  ;; return-unmemo: return ANS (and memo table if applicable) without updating memo table
+  ;; return-memo: return ANS while updating memo table
+  ;; bind: bind ANS (and memo table if applicable) to return of recursive call
+  ;; memo-lookup: b* binders for looking up id in memo table and returning if available
+  '(define fnname ((id natp)
+                   aignet
+                   pathcond-nodestack
+                   pathcond-nodebits
+                   . memo-args)
+     :guard (and (< id (num-fanins aignet))
+                 (< id (bits-length pathcond-nodebits))
+                 . memo-guard)
+     :returns returns
+     :measure (nfix id)
+     :verify-guards nil
+     (b* ((id (lnfix id))
+          ((when (eql id 0))
+           (b* ((ans 0)) return-unmemo))
+          (boundp (acl2::intstack-member^ id pathcond-nodestack))
+          ((when boundp)
+           (b* ((ans (get-bit id pathcond-nodebits)))
+             return-unmemo))
+          (slot0 (id->slot0 id aignet))
+          (type (snode->type^ slot0))
+          ((unless (eql type (gate-type)))
+           (b* ((ans nil))
+             return-unmemo)))
+       (b* memo-lookup
+         (b* ((fanin0 (snode->fanin^ slot0))
+              (bind (fnname (lit->var fanin0)
+                            aignet pathcond-nodestack pathcond-nodebits . memo-args))
+              (f0-res ans)
+              (slot1 (id->slot1 id aignet))
+              (and-gate-p (eql (snode->regp^ slot1) 0))
+              ((when (and f0-res
+                          (eql (b-xor f0-res (lit->neg fanin0)) 0)
+                          and-gate-p))
+               (b* ((ans 0))
+                 return-memo))
+              ((when (and (not f0-res) (not and-gate-p)))
+               (b* ((ans nil))
+                 return-memo))
+              (fanin1 (snode->fanin^ slot1))
+              (bind (fnname (lit->var fanin1)
+                            aignet pathcond-nodestack pathcond-nodebits . memo-args))
+              (f1-res ans)
+              ((when (and f1-res
+                          (eql (b-xor f1-res (lit->neg fanin1)) 0)
+                          and-gate-p))
+               (b* ((ans 0))
+                 return-memo))
+              ((unless (and f0-res f1-res))
+               (b* ((ans nil))
+                 return-memo))
+              (ans (if and-gate-p
+                       1 ;; (b-and f0-res f1-res)
+                     (b-xor (b-xor f0-res (lit->neg fanin0))
+                            (b-xor f1-res (lit->neg fanin1))))))
+           return-memo)))
+     ///
+     (local (in-theory (disable (:d fnname))))
+     (verify-guards fnname)))
+
+(define aignet-pathcond-implies-memo-get ((var natp)
+                                          pathcond-memo)
+  :inline t
+  :returns (mv set (val acl2::maybe-bitp :rule-classes :type-prescription))
+  :guard (< (+ 1 (* 2 var)) (eba-length pathcond-memo))
+  (b* ((memo-bit1 (eba-get-bit (* 2 (the integer (lnfix var))) pathcond-memo))
+       (memo-bit0 (eba-get-bit (+ 1 (* 2 (the integer (lnfix var)))) pathcond-memo))
+       ((unless (or (eql memo-bit1 1) (eql memo-bit0 1))) (mv nil 0))
+       ((when (eql memo-bit1 memo-bit0)) (mv t nil)))
+    (mv t memo-bit1)))
+
+(define aignet-pathcond-implies-memo-set ((var natp)
+                                          (val acl2::maybe-bitp)
+                                          pathcond-memo)
+  :inline t
+  :returns new-pathcond-memo
+  :guard (< (+ 1 (* 2 var)) (eba-length pathcond-memo))
+  (case (acl2::maybe-bit-fix val)
+    (1 (b* ((pathcond-memo (eba-set-bit (* 2 (the integer (lnfix var))) pathcond-memo)))
+         (eba-clear-bit (+ 1 (* 2 (the integer (lnfix var)))) pathcond-memo)))
+    (0 (b* ((pathcond-memo (eba-clear-bit (* 2 (the integer (lnfix var))) pathcond-memo)))
+         (eba-set-bit (+ 1 (* 2 (the integer (lnfix var)))) pathcond-memo)))
+    (t (b* ((pathcond-memo (eba-set-bit (* 2 (the integer (lnfix var))) pathcond-memo)))
+         (eba-set-bit (+ 1 (* 2 (the integer (lnfix var)))) pathcond-memo))))
+  ///
+  (defret aignet-pathcond-implies-memo-get-of-memo-set
+    (equal (aignet-pathcond-implies-memo-get var1 new-pathcond-memo)
+           (if (equal (nfix var1) (nfix var))
+               (mv t (acl2::maybe-bit-fix val))
+             (aignet-pathcond-implies-memo-get var1 pathcond-memo)))
+    :hints(("Goal" :in-theory (enable aignet-pathcond-implies-memo-get
+                                      maybe-bit-fix))))
+
+  ;; (local (in-theory (enable aignet-pathcond-implies-memo-get-of-memo-set)))
+
+  ;; (defret aignet-pathcond-implies-memo-get-of-memo-set-same
+  ;;   (equal (aignet-pathcond-implies-memo-get var new-pathcond-memo)
+  ;;          (mv t (acl2::maybe-bit-fix val)))
+  ;;   :hints(("Goal" :in-theory (disable aignet-pathcond-implies-memo-set))))
+
+  ;; (defret aignet-pathcond-implies-memo-get-of-memo-set-diff
+  ;;   (implies (not (equal (nfix var1) (nfix var)))
+  ;;            (equal (aignet-pathcond-implies-memo-get var1 new-pathcond-memo)
+  ;;                   (aignet-pathcond-implies-memo-get var1 pathcond-memo)))
+  ;;   :hints(("Goal" :in-theory (disable aignet-pathcond-implies-memo-set))))
+
+  (defret len-memo-of-<fn>
+    (implies (< (+ 1 (* 2 (nfix var))) (len pathcond-memo))
+             (equal (len new-pathcond-memo) (len pathcond-memo)))))
+
+
+(defsection aignet-pathcond-implies
+  (make-event
+   (sublis
+    '((fnname . aignet-pathcond-implies) ;; fnname: obvious
+      (memo-args . nil) ;; memo-args: memo tables to pass around
+      (memo-guard . nil) ;; memo-guard: list of conjuncts for guard of memo-args
+      (returns . (ans acl2::maybe-bitp :rule-classes :type-prescription)) ;; returns: :returns entry
+      (return-unmemo . ans) ;; return-unmemo: return ANS (and memo table if applicable) without updating memo table
+      (return-memo . ans) ;; return-memo: return ANS while updating memo table
+      (bind . ans) ;; bind: bind ANS (and memo table if applicable) to return of recursive call
+      (memo-lookup . nil)) ;; memo-lookup: b* binders for looking up id in memo table and returning if available
+    *aignet-pathcond-implies-template*))
+  
+  (local (in-theory (enable (:i aignet-pathcond-implies))))
+
+  (
+
+
+
+
+  )
+
+(local (defthm bitp-when-maybe-bitp
+         (implies (and x (acl2::maybe-bitp x))
+                  (bitp x))))
+
+(defsection aignet-pathcond-implies-memo
+  (make-event
+   (sublis
+    '((fnname . aignet-pathcond-implies-memo) ;; fnname: obvious
+      (memo-args . (pathcond-memo)) ;; memo-args: memo tables to pass around
+      ;; memo-guard: list of conjuncts for guard of memo-args
+      (memo-guard . ((< (+ 1 (* 2 id)) (eba-length pathcond-memo))))
+      ;; returns: :returns entry
+      (returns . (mv (ans acl2::maybe-bitp :rule-classes :type-prescription)
+                     (new-pathcond-memo
+                      (implies (< (+ 1 (* 2 (nfix id))) (len pathcond-memo))
+                               (equal (len new-pathcond-memo) (len pathcond-memo))))))
+      ;; return-unmemo: return ANS (and memo table if applicable) without updating memo table
+      (return-unmemo . (mv ans pathcond-memo))
+      ;; return-memo: return ANS while updating memo table
+      (return-memo . (b* ((pathcond-memo (aignet-pathcond-implies-memo-set id ans pathcond-memo)))
+                       (mv ans pathcond-memo)))
+      ;; bind: bind ANS (and memo table if applicable) to return of recursive call
+      (bind . (mv ans pathcond-memo))
+      ;; memo-lookup: b* binders for looking up id in memo table and returning if available
+      (memo-lookup . (((mv set ans) (aignet-pathcond-implies-memo-get id pathcond-memo))
+                      ((when set) (mv ans pathcond-memo)))))
+    *aignet-pathcond-implies-template*))
+
+  (local (in-theory (enable (:i aignet-pathcond-implies-memo))))
+
+
+  (defun-sk aignet-pathcond-implies-memo-cond (aignet
+                                               pathcond-nodestack
+                                               pathcond-nodebits
+                                               pathcond-memo)
+    (forall id
+            (b* (((mv memo-set memo-val) (aignet-pathcond-implies-memo-get
+                                          id pathcond-memo)))
+              (implies memo-set
+                       (equal memo-val
+                              (aignet-pathcond-implies id aignet pathcond-nodestack pathcond-nodebits)))))
+    :rewrite :direct)
+
+  (local (in-theory (disable aignet-pathcond-implies-memo-cond
+                             b-xor not)))
+
+  (defret aignet-pathcond-implies-memo-correct
+    (implies (aignet-pathcond-implies-memo-cond aignet pathcond-nodestack pathcond-nodebits
+                                                pathcond-memo)
+             (and (equal ans (aignet-pathcond-implies id aignet pathcond-nodestack pathcond-nodebits))
+                  (aignet-pathcond-implies-memo-cond aignet pathcond-nodestack pathcond-nodebits new-pathcond-memo)))
+    :hints (("goal" :induct <call>)
+            (and stable-under-simplificationp
+                 (b* ((lit (assoc 'aignet-pathcond-implies-memo-cond clause))
+                      (expands '(:expand (<call>
+                                          (aignet-pathcond-implies
+                                           id aignet pathcond-nodestack pathcond-nodebits)
+                                          (aignet-pathcond-implies
+                                           0 aignet pathcond-nodestack pathcond-nodebits)
+                                          (aignet-pathcond-implies-memo
+                                           0 aignet pathcond-nodestack pathcond-nodebits pathcond-memo)))))
+                   (if lit
+                       `(:computed-hint-replacement
+                         ((and stable-under-simplificationp
+                               ',expands))
+                         :expand (,lit)
+                         :do-not-induct t)
+                     expands)))))
+
+
+  (defthm aignet-pathcond-implies-memo-cond-of-repeat-0
+    (aignet-pathcond-implies-memo-cond aignet
+                                       pathcond-nodestack
+                                       pathcond-nodebits
+                                       (acl2::repeat n 0))
+    :hints(("Goal" :in-theory (enable aignet-pathcond-implies-memo-cond
+                                      aignet-pathcond-implies-memo-get)))))
+
+
+
+
+                                               
+        
+
+
